Foundation/Propositional/Kripke2/Hilbert/F_Rfl_Sym.lean
@@ -1,13 +1,12 @@
 module
 
-public import Foundation.Propositional.Kripke2.Logic.F_Rfl
-public import Foundation.Propositional.Kripke2.Logic.F_Sym
+public import Foundation.Propositional.Kripke2.Hilbert.F_Rfl
+public import Foundation.Propositional.Kripke2.Hilbert.F_Sym
 
 @[expose] public section
 
 namespace LO.Propositional
 
-open Hilbert.F
 open Kripke2
 
 
@@ -21,28 +20,27 @@ instance : trivialFrame.IsF_Rfl_Sym where
 end Kripke2
 
 
-namespace F_Rfl_Sym
+namespace HilbertF.F_Rfl_Sym
 
-open Hilbert.F.Kripke2
+open Kripke2
 
-instance Kripke2.sound : Sound Propositional.F_Rfl_Sym FrameClass.F_Rfl_Sym := by
+instance soundKripke2 : Sound (HilbertF.F_Rfl_Sym : HilbertF ℕ) ({ F | F.IsF_Rfl_Sym } : Kripke2.FrameClass) := by
   apply instFrameClassSound;
   constructor;
   rintro φ hφ F hF;
   replace hF := Set.mem_setOf_eq.mp hF;
   rcases hφ with (⟨_, _, _, rfl⟩ | ⟨_, _, _, rfl⟩) <;> simp;
 
-instance : Entailment.Consistent Propositional.F_Rfl_Sym := consistent_of_sound_frameclass FrameClass.F_Rfl_Sym $ by
+instance : Entailment.Consistent (HilbertF.F_Rfl_Sym : HilbertF ℕ) := consistent_of_sound_frameclass soundKripke2 $ by
   use Kripke2.trivialFrame;
   apply Set.mem_setOf_eq.mpr;
   infer_instance;
 
-end F_Rfl_Sym
+end HilbertF.F_Rfl_Sym
 
-instance : Propositional.F_Rfl ⪱ Propositional.F_Rfl_Sym := by
+instance : (HilbertF.F_Rfl : HilbertF ℕ) ⪱ HilbertF.F_Rfl_Sym := by
   constructor;
-  . apply weakerThan_of_subset_axioms;
-    simp;
+  . grind;
   . apply Entailment.not_weakerThan_iff.mpr;
     use (Axioms.Sym #0 #1);
     constructor;
@@ -57,15 +55,14 @@ instance : Propositional.F_Rfl ⪱ Propositional.F_Rfl_Sym := by
         have := isSymmetric_of_valid_axiomSym hC |>.symm 0 1;
         grind;
 
-instance : Propositional.F_Sym ⪱ Propositional.F_Rfl_Sym := by
+instance : (HilbertF.F_Sym : HilbertF ℕ) ⪱ HilbertF.F_Rfl_Sym := by
   constructor;
-  . apply weakerThan_of_subset_axioms;
-    simp;
+  . grind;
   . apply Entailment.not_weakerThan_iff.mpr;
     use (Axioms.Rfl #0 #1);
     constructor;
     . simp;
-    . apply Sound.not_provable_of_countermodel (𝓜 := Kripke2.FrameClass.F_Sym);
+    . apply Sound.not_provable_of_countermodel (𝓜 := ({ F | F.IsSymmetric } : Kripke2.FrameClass));
       apply Kripke2.not_validOnFrameClass_of_exists_frame;
       use ⟨Fin 2, (λ x y => x = 0 ∨ x ≠ y), 0, by simp⟩;
       constructor;
