Foundation/Propositional/Kripke2/Hilbert/F_Rfl_Tra1.lean
@@ -1,13 +1,12 @@
 module
 
-public import Foundation.Propositional.Kripke2.Logic.F_Rfl
-public import Foundation.Propositional.Kripke2.Logic.F_Tra1
+public import Foundation.Propositional.Kripke2.Hilbert.F_Rfl
+public import Foundation.Propositional.Kripke2.Hilbert.F_Tra1
 
 @[expose] public section
 
 namespace LO.Propositional
 
-open Hilbert.F
 open Kripke2
 
 
@@ -21,28 +20,27 @@ instance : trivialFrame.IsF_Rfl_Tra1 where
 end Kripke2
 
 
-namespace F_Rfl_Tra1
+namespace HilbertF.F_Rfl_Tra1
 
-open Hilbert.F.Kripke2
+open Kripke2
 
-instance Kripke2.sound : Sound Propositional.F_Rfl_Tra1 FrameClass.F_Rfl_Tra1 := by
+instance soundKripke2 : Sound (HilbertF.F_Rfl_Tra1 : HilbertF ℕ) ({ F | F.IsF_Rfl_Tra1 } : Kripke2.FrameClass) := by
   apply instFrameClassSound;
   constructor;
   rintro φ hφ F hF;
   replace hF := Set.mem_setOf_eq.mp hF;
   rcases hφ with (⟨_, _, _, rfl⟩ | ⟨_, _, _, rfl⟩) <;> simp;
 
-instance : Entailment.Consistent Propositional.F_Rfl_Tra1 := consistent_of_sound_frameclass FrameClass.F_Rfl_Tra1 $ by
+instance : Entailment.Consistent (HilbertF.F_Rfl_Tra1 : HilbertF ℕ) := consistent_of_sound_frameclass soundKripke2 $ by
   use Kripke2.trivialFrame;
   apply Set.mem_setOf_eq.mpr;
   infer_instance;
 
-end F_Rfl_Tra1
+end HilbertF.F_Rfl_Tra1
 
-instance : Propositional.F_Rfl ⪱ Propositional.F_Rfl_Tra1 := by
+instance : (HilbertF.F_Rfl : HilbertF ℕ) ⪱ HilbertF.F_Rfl_Tra1 := by
   constructor;
-  . apply weakerThan_of_subset_axioms;
-    simp;
+  . grind;
   . apply Entailment.not_weakerThan_iff.mpr;
     use (Axioms.Tra1 #0 #1 #2);
     constructor;
@@ -57,10 +55,9 @@ instance : Propositional.F_Rfl ⪱ Propositional.F_Rfl_Tra1 := by
         have := IsTransitive_of_valid_axiomTra₁ hC |>.trans 1 2 3 (by omega) (by omega);
         grind;
 
-instance : Propositional.F_Tra1 ⪱ Propositional.F_Rfl_Tra1 := by
+instance : (HilbertF.F_Tra1 : HilbertF ℕ) ⪱ HilbertF.F_Rfl_Tra1 := by
   constructor;
-  . apply weakerThan_of_subset_axioms;
-    simp;
+  . grind;
   . apply Entailment.not_weakerThan_iff.mpr;
     use (Axioms.Rfl #0 #1);
     constructor;
