Foundation/Propositional/Kripke2/Axiom/Rfl.lean
@@ -1,6 +1,6 @@
 module
 
-public import Foundation.Propositional.Kripke2.AxiomSer
+public import Foundation.Propositional.Kripke2.Axiom.Ser
 
 @[expose] public section
 
@@ -43,12 +43,6 @@ lemma isReflexive_of_valid_axiomRfl (h : F ⊧ Axioms.Rfl #0 #1) : F.IsReflexive
     . rintro y Rxy;
       tauto;
   exact this;
-
-instance [Entailment.F L] [Entailment.HasAxiomRfl L] [Entailment.Disjunctive L] : Frame.IsReflexive (canonicalModel L).toFrame where
-  refl := by
-    rintro T φ ψ hφψ hφ;
-    apply T.imp_closed (show L ⊢ Axioms.Rfl φ ψ from by simp);
-    apply T.andIR <;> assumption;
 
 end Kripke2
 
